coq_translation/examples-from-rust-book/variable_bindings/declare_first.v
@@ -6,7 +6,7 @@ Import Root.std.prelude.rust_2015.
 Definition main (_ : unit) : unit :=
   let a_binding := tt in
   let x := 2 in
-  assign a_binding := mul x x ;;
+  assign a_binding (mul x x) ;;
   tt ;;
   _crate.io._print
     (_crate.fmt.ImplArguments.new_v1
@@ -14,7 +14,7 @@ Definition main (_ : unit) : unit :=
       [ _crate.fmt.ImplArgumentV1.new_display a_binding ]) ;;
   tt ;;
   let another_binding := tt in
-  assign another_binding := 1 ;;
+  assign another_binding 1 ;;
   _crate.io._print
     (_crate.fmt.ImplArguments.new_v1
       [ "another binding: "; "\n" ]
